Better version of linearize without a-normal form
Now we no longer let-bind arguments to Op (oops)

src/Compilers/Linearize.v
@@ -20,34 +20,48 @@ Section language.
     Local Notation expr := (@expr base_type_code op var).
 
     Section under_lets.
-      Fixpoint under_letsf {t} (e : exprf t)
-        : forall {tC} (C : interp_flat_type var t -> exprf tC), exprf tC
-        := match e in Syntax.exprf _ _ t return forall {tC} (C : interp_flat_type var t -> exprf tC), exprf tC with
+      Fixpoint under_letsf' {t} (e : exprf t)
+        : forall {tC} (C : interp_flat_type var t + exprf t -> exprf tC), exprf tC
+        := match e in Syntax.exprf _ _ t return forall {tC} (C : interp_flat_type var t + exprf t -> exprf tC), exprf tC with
            | LetIn _ ex _ eC
-             => fun _ C => @under_letsf _ ex _ (fun v => @under_letsf _ (eC v) _ C)
-           | TT => fun _ C => C tt
-           | Var _ x => fun _ C => C x
-           | Op _ _ op args as e => fun _ C => LetIn e C
-           | Pair A x B y => fun _ C => @under_letsf A x _ (fun x =>
-                                        @under_letsf B y _ (fun y =>
-                                        C (x, y)))
+             => fun _ C => @under_letsf' _ ex _ (fun v =>
+                           match v with
+                           | inl v => @under_letsf' _ (eC v) _ C
+                           | inr v => LetIn v (fun v => @under_letsf' _ (eC v) _ C)
+                           end)
+           | TT => fun _ C => C (inl tt)
+           | Var _ x => fun _ C => C (inl x)
+           | Op _ _ op args as e
+             => if let_bind_op_args
+                then fun _ C => LetIn e (fun v => C (inl v))
+                else fun _ C => C (inr e)
+           | Pair A x B y => fun _ C => @under_letsf' A x _ (fun x =>
+                                        @under_letsf' B y _ (fun y =>
+                                        match x, y with
+                                        | inl x, inl y => C (inl (x, y))
+                                        | inl x, inr y => C (inr (Pair (SmartVarf x) y))
+                                        | inr x, inl y => C (inr (Pair x (SmartVarf y)))
+                                        | inr x, inr y => C (inr (Pair x y))
+                                        end))
            end.
+      Definition under_letsf {t} (e : exprf t)
+                 {tC} (C : exprf t -> exprf tC)
+        : exprf tC
+        := under_letsf' e (fun v => match v with inl v => C (SmartVarf v) | inr v => C v end).
     End under_lets.
 
     Fixpoint linearizef_gen {t} (e : exprf t) : exprf t
       := match e in Syntax.exprf _ _ t return exprf t with
          | LetIn _ ex _ eC
-           => under_letsf (@linearizef_gen _ ex) (fun x => @linearizef_gen _ (eC x))
+           => under_letsf (LetIn (@linearizef_gen _ ex) (fun x => @linearizef_gen _ (eC x))) (fun x => x)
          | TT => TT
          | Var _ x => Var x
          | Op _ _ op args
            => if let_bind_op_args
-              then under_letsf (@linearizef_gen _ args) (fun args => LetIn (Op op (SmartVarf args)) SmartVarf)
-              else Op op (@linearizef_gen _ args)
+              then under_letsf (@linearizef_gen _ args) (fun args => LetIn (Op op args) SmartVarf)
+              else under_letsf (@linearizef_gen _ args) (fun args => Op op args)
          | Pair A ex B ey
-           => under_letsf (@linearizef_gen _ ex) (fun x =>
-              under_letsf (@linearizef_gen _ ey) (fun y =>
-              SmartVarf (t:=Prod A B) (x, y)))
+           => under_letsf (Pair (@linearizef_gen _ ex) (@linearizef_gen _ ey)) (fun v => v)
          end.
 
     Definition linearize_gen {t} (e : expr t) : expr t
@@ -60,7 +74,8 @@ Section language.
     := fun var => linearize_gen (e _).
 End language.
 
-Global Arguments under_letsf {_ _ _ _} _ {tC} _.
+Global Arguments under_letsf' _ {_ _ _ _} _ {tC} _.
+Global Arguments under_letsf _ {_ _ _ _} _ {tC} _.
 Global Arguments linearizef_gen _ {_ _ _ _} _.
 Global Arguments linearize_gen _ {_ _ _ _} _.
 Global Arguments Linearize_gen _ {_ _ _} _ var.
